abstract_machine_facts.v
@@ -1,0 +1,114 @@
+Require Import abstract_machine.
+
+
+Module DetAbstractMachine_Sim (AM : DET_ABSTRACT_MACHINE).
+
+  Import AM.
+
+
+  Fixpoint n_steps c n : option configuration :=
+      match n with
+      | 0   => Some c
+      | S n => match next_conf c with
+               | None    => None
+               | Some c' => n_steps c' n
+               end
+      end.
+
+
+  Lemma n_steps_correct : forall c1 n c2, n_steps c1 (S n) = Some c2 -> c1 →+ c2.
+
+  Proof.
+    intros c1 n c2; revert c1.
+
+    induction n; 
+        intros c1 H;
+        remember (next_conf c1) as c1'; destruct c1';
+        simpl in H;
+        rewrite <- Heqc1' in *;
+        try discriminate.
+
+    - constructor 1.
+      apply next_correct. 
+      congruence.
+    - econstructor 2.
+      + apply next_correct. 
+        symmetry; exact Heqc1'.
+      + apply IHn.
+        simpl; auto.
+  Qed.
+
+
+  Lemma n_steps_complete : 
+      forall c1 c2,  c1 →+ c2  -> exists n, n_steps c1 n = Some c2.
+
+  Proof.
+    induction 1.
+    - exists 1; simpl. 
+      apply next_correct in H.
+      rewrite H; auto.
+    - destruct IHtrans_close as (n, H1).
+      apply next_correct in H.
+      eexists (S n).
+      simpl.
+      rewrite H; auto.
+  Qed.
+
+
+(* BEGINE Hell
+
+  Axiom conf_eq_dec : forall c1 c2 : configuration, {c1 = c2} + {c1 <> c2}.
+
+  Definition steps_count c1 c2 (H : c1 →+ c2) : nat.
+    refine (
+     (fix aux c1 c2 (H : c1 →+ c2) {struct H} :=
+      match next_conf c1 as c' return next_conf c1 = c' -> nat with
+      | None    => fun _ => _
+      | Some c' => fun G => if conf_eq_dec c' c2 then 1
+                            else S (aux c' c2 _)
+      end eq_refl)
+      c1 c2 H).
+  - destruct H0 as [? ? H0 | ? ? ? H0 ?];
+        apply next_correct in H0;
+        rewrite H0 in G; inversion G; subst;
+    solve [tauto].
+  - contradict _H.
+    destruct H0 as [? ? H0 | ? ? ? H0 ?];
+        apply next_correct in H0;
+        rewrite H0;
+    solve [discriminate].
+  Defined.
+
+
+  Require Import Program.
+(*
+  Lemma L : forall c1 c2 (H : c1 →+ c2),
+                steps_count c1 c2 H <> 0.
+  Proof.
+    intros c1 c2 H.
+    destruct H.
+    simpl.
+    remember (next_conf c1).
+    dependent destruction (next_conf c1).
+*)
+  Lemma steps_count_correct : 
+      forall c1 c2 (H : c1 →+ c2), n_steps c1 (steps_count c1 c2 H) = Some c2.
+
+  Proof.
+    intros c1 c2 H.
+    remember (steps_count c1 c2 H) as n.
+    induction n.
+    destruct H as [? ? H | ? ? ? H H'];
+        assert (HH := H);
+        apply next_correct in HH.
+    + simpl in Heqn.
+      rewrite HH in Heqn.
+    
+    remember (next_conf c1) as c'.
+    destruct c
+
+END Hell *)
+
+End DetAbstractMachine_Sim.
+
+  
